# Exercise 1

$$
\begin{align}
(212)_3 \cdot (122)_3 &= (2 \cdot 3^2 + 1 \cdot 3 + 2) \cdot (1 \cdot 3^2 + 2 \cdot 3 + 2) \\
                      &= (2 \cdot 3^4 + 1 \cdot 3^3 + 2 \cdot 3^2) + (4 \cdot 3^3 + 2 \cdot 3^2 + 4 \cdot 3) + (4 \cdot 3^2 + 2 \cdot 3 + 4) \\
                      &= 2 \cdot 3^4 + 5 \cdot 3^3 + 8 \cdot 3^2 + 6 \cdot 3 + 4 \\
                      &= 2 \cdot 3^4 + (3 + 2) \cdot 3^3 + (2 \cdot 3 + 2) \cdot 3^2 + (2 \cdot 3) \cdot 3 + 3 + 1 \\
                      &= 2 \cdot 3^4 + 3^4 + 2 \cdot 3^3 + 2 \cdot 3^3 + 2 \cdot 3^2 + 2 \cdot 3^2 + 3 + 1 \\
                      &= 3 \cdot 3^4 + 4 \cdot 3^3 + 4 \cdot 3^2 + 2 \cdot 3^2 + 3 + 1 \\
                      &= 
\end{align}
$$
